GRAT version 1.2. New optimizations, now more than 2x fatsre than drat-trim

GRAT/gratchk/code/bin_reader.sml
@@ -1,0 +1,94 @@
+(*
+  Buffered reader to expose a file of 
+  little-endian int32 values as a stream in 
+  reverse order, i.e., the last int is read first.
+*)
+signature BIN_READER = sig
+  (* Type of stream *)
+  type rd
+  (* Exception to be thrown on error *)
+  exception Err of string
+  (* Open a file *)
+  val openf : string -> Position.int * rd
+  (* Read a signed 32 bit integer, and return as int *)
+  val rd32 : rd -> int * rd
+  (* Check if end of stream (beginning of file) has been reached *)
+  val at_end : rd -> bool
+  
+  (* Get position where last int has been read from. At least one int must have been read for this to be accurate! *)
+  val last_rd_pos : rd -> Position.int
+end
+
+structure Bin_Reader : BIN_READER = struct
+  type rd = { 
+    buf_start_pos : Position.int,
+    in_buf_pos : int,
+    buf : Word8ArraySlice.slice,
+    fd : Posix.IO.file_desc
+  }
+
+  exception Err of string
+
+  val buf_size = ref (Position.fromInt 65536)
+  
+  fun openf name = let
+    open Posix
+    val fd = FileSys.openf(name,FileSys.O_RDONLY,FileSys.O.nonblock) 
+    val st = FileSys.fstat fd
+    val size = FileSys.ST.size st
+    
+    val buf_start_pos = if size=0 then 0 else (Position.div (size - 1, !buf_size) + 1) * (!buf_size)
+    
+    val arr = Word8Array.array(Position.toInt (!buf_size), Word8.fromInt 0)
+    val arrsl = Word8ArraySlice.slice(arr,0,NONE)
+    
+  in
+    ( size,
+      {
+        buf_start_pos = buf_start_pos,
+        in_buf_pos = 0,
+        buf = arrsl,
+        fd=fd
+      }
+    )
+  end
+
+  fun prepare_rd (rd as {buf_start_pos, in_buf_pos, buf, fd}) = 
+    if in_buf_pos = 0 then 
+      let
+        val _ = buf_start_pos >= !buf_size orelse raise Err "Read beyond start of file"
+        val buf_start_pos = buf_start_pos - !buf_size
+        val xxpos = Posix.IO.lseek (fd,buf_start_pos,Posix.IO.SEEK_SET)
+        val _ = xxpos = buf_start_pos orelse raise Err "Invalid seek pos"
+        val in_buf_pos = Posix.IO.readArr (fd,buf)
+        val _ = in_buf_pos > 0 orelse raise Err "Read 0 bytes?"
+      in
+        {buf_start_pos = buf_start_pos,in_buf_pos = in_buf_pos, buf = buf, fd = fd}
+      end
+    else
+      rd
+  
+  fun rd32 rd = let
+    val {buf_start_pos, in_buf_pos, buf, fd} = prepare_rd rd
+    val _ = in_buf_pos >= 4 orelse raise Err "Unaligned in-buf-pos?"
+    val in_buf_pos = in_buf_pos - 4
+    val b1 = Word8.toLarge (Word8ArraySlice.sub (buf,in_buf_pos + 0))
+    val b2 = Word8.toLarge (Word8ArraySlice.sub (buf,in_buf_pos + 1))
+    val b3 = Word8.toLarge (Word8ArraySlice.sub (buf,in_buf_pos + 2))
+    val b4 = Word8.toLarge (Word8ArraySlice.sub (buf,in_buf_pos + 3))
+
+    val res = Word32.fromLarge (b1 + LargeWord.<<(b2, Word.fromInt 8) + LargeWord.<<(b3, Word.fromInt 16) + LargeWord.<<(b4, Word.fromInt 24))
+    val res = Word32.toIntX res 
+    val rd = {buf_start_pos = buf_start_pos,in_buf_pos = in_buf_pos, buf = buf, fd = fd}
+  in
+    (res, rd)
+  end
+  
+  
+  fun at_end {buf_start_pos, in_buf_pos, buf, fd} = buf_start_pos = Position.fromInt 0 andalso in_buf_pos = 0
+  
+  fun last_rd_pos {buf_start_pos, in_buf_pos, buf, fd} = buf_start_pos + Position.fromInt in_buf_pos
+  
+  
+  
+end
