GRAT/gratchk/code/gratchk_export.sml
@@ -301,6 +301,13 @@ structure Grat_Check : sig
   val verify_unsat_impl_wrapper :
     int array ->
       nat -> nat -> (unit -> ((string * (int option * nat option)), unit) sum)
+  val verify_unsat_split_impl_wrapper :
+    int array ->
+      ('a -> int * 'a) ->
+        nat ->
+          nat ->
+            nat * 'a ->
+              (unit -> ((string * (int option * (nat * 'a) option)), unit) sum)
 end = struct
 
 datatype typerepa = Typerep of string * typerepa list;
@@ -591,6 +598,11 @@ fun array_grow A_ a s x =
 fun mbhd_insert A_ x l =
   (if null l then [x] else (if eq A_ x (hd l) then l else x :: l));
 
+val creg_dflt_size : nat = nat_of_integer (16 : IntInf.int);
+
+val creg_empty : (unit -> (((nat list) option) array)) =
+  new (heap_option (heap_list heap_nat)) creg_dflt_size NONE;
+
 val assignment_empty_impl : (unit -> (nat array)) =
   new heap_nat (nat_of_integer (16 : IntInf.int)) zero_nat;
 
@@ -702,6 +714,8 @@ fun verify_sat3 x =
     end)
     x;
 
+fun at_item_end frml_end it = less_eq_nat it frml_end;
+
 fun imp_nfoldli (x :: ls) c f s =
   (fn () =>
     let
@@ -719,11 +733,6 @@ fun unset_var_impl x =
 fun backtrack3 x =
   (fn ai => fn bi => imp_nfoldli bi (fn _ => (fn () => true)) unset_var_impl ai)
     x;
-
-val creg_dflt_size : nat = nat_of_integer (16 : IntInf.int);
-
-val creg_empty : (unit -> (((nat list) option) array)) =
-  new (heap_option (heap_list heap_nat)) creg_dflt_size NONE;
 
 fun less_eq_int k l = IntInf.<= (integer_of_int k, integer_of_int l);
 
@@ -777,8 +786,6 @@ fun add_clause3 x =
            end)
     end)
     x;
-
-fun at_item_end frml_end it = less_eq_nat it frml_end;
 
 fun check_conflict_clause3 x =
   (fn ai => fn bib => fn bia => fn bi => fn () =>
@@ -1652,6 +1659,72 @@ fun apply_units3 x =
     end)
     x;
 
+fun remove_ids3 x =
+  (fn ai => fn bia => fn bi => fn () =>
+    let
+      val xa = len heap_int ai ();
+    in
+      (if not (equal_nata bi xa)
+        then (fn f_ => fn () => f_
+               ((heap_WHILET
+                  (fn a =>
+                    (case a of Inl _ => (fn () => false)
+                      | Inr (_, a2) =>
+                        (fn f_ => fn () => f_ ((nth heap_int ai a2) ()) ())
+                          (fn xb => (fn () => (not (equal_int xb zero_int))))))
+                  (fn s =>
+                    let
+                      val (a1, a2) = projr s;
+                    in
+                      (fn f_ => fn () => f_ ((len heap_int ai) ()) ())
+                        (fn xb =>
+                          (if not (equal_nata a2 xb)
+                            then (fn f_ => fn () => f_ ((nth heap_int ai a2) ())
+                                   ())
+                                   (fn xc =>
+                                     (fn f_ => fn () => f_
+                                       ((if less_int zero_int xc
+  then (fn f_ => fn () => f_ ((nth heap_int ai a2) ()) ())
+         (fn xd => (fn () => (Inr (nat xd, plus_nat one_nat a2))))
+  else (fn f_ => fn () => f_ ((nth heap_int ai a2) ()) ())
+         (fn xd => (fn () => (Inl ("Invalid id", (SOME xd, SOME a2))))))
+                                       ()) ())
+                                       (fn a =>
+ (case a of Inl x1a => (fn () => (Inl x1a))
+   | Inr (a1a, a2a) =>
+     (fn f_ => fn () => f_ ((len heap_int ai) ()) ())
+       (fn xd =>
+         (if not (equal_nata a2a xd)
+           then (fn f_ => fn () => f_
+                  (let
+                     val (a1b, a2b) = a1;
+                   in
+                     (fn f_ => fn () => f_
+                       ((array_set_dyn heap_nat zero_nat a1b a1a zero_nat) ())
+                       ())
+                       (fn x_g => (fn () => (x_g, a2b)))
+                   end
+                  ()) ())
+                  (fn x_g => (fn () => (Inr (x_g, a2a))))
+           else (fn () => (Inl ("Parsed beyond end", (NONE, NONE)))))))))
+                            else (fn () =>
+                                   (Inl ("Parsed beyond end", (NONE, NONE))))))
+                    end)
+                  (Inr (bia, bi)))
+               ()) ())
+               (fn a =>
+                 (case a of Inl x1a => (fn () => (Inl x1a))
+                   | Inr (a1, a2) =>
+                     (fn f_ => fn () => f_ ((len heap_int ai) ()) ())
+                       (fn xb =>
+                         (fn () =>
+                           (if not (equal_nata a2 xb) then Inr a1
+                             else Inl ("Parsed beyond end", (NONE, NONE)))))))
+        else (fn () => (Inl ("Parsed beyond end", (NONE, NONE)))))
+        ()
+    end)
+    x;
+
 fun check_item3 x =
   (fn ai => fn bia => fn bi =>
     let
@@ -1694,44 +1767,10 @@ fun check_item3 x =
                                else (if equal_nata a1b
   (nat_of_integer (2 : IntInf.int))
                                       then (fn f_ => fn () => f_
-     ((len heap_int ai) ()) ())
-     (fn xc =>
-       (if not (equal_nata a2b xc)
-         then (fn f_ => fn () => f_ ((nth heap_int ai a2b) ()) ())
-                (fn xd =>
-                  (fn f_ => fn () => f_
-                    ((if less_int zero_int xd
-                       then (fn f_ => fn () => f_ ((nth heap_int ai a2b) ()) ())
-                              (fn xe =>
-                                (fn () => (Inr (nat xe, plus_nat one_nat a2b))))
-                       else (fn f_ => fn () => f_ ((nth heap_int ai a2b) ()) ())
-                              (fn xe =>
-                                (fn () =>
-                                  (Inl ("Invalid id", (SOME xe, SOME a2b))))))
-                    ()) ())
-                    (fn aa =>
-                      (case aa of Inl x1a => (fn () => (Inl x1a))
-                        | Inr x2aa =>
-                          (fn f_ => fn () => f_
-                            (let
-                               val (a1c, _) = x2aa;
-                             in
-                               (fn f_ => fn () => f_
-                                 (let
-                                    val (a1d, a2d) = a1a;
-                                  in
-                                    (fn f_ => fn () => f_
-                                      ((array_set_dyn heap_nat zero_nat a1d a1c
- zero_nat)
-                                      ()) ())
-                                      (fn x_h => (fn () => (x_h, a2d)))
-                                  end
-                                 ()) ())
-                                 (fn x_h => (fn () => (SOME (a1, (x_h, a2a)))))
-                             end
-                            ()) ())
-                            (fn x_h => (fn () => (Inr x_h))))))
-         else (fn () => (Inl ("Parsed beyond end", (NONE, NONE))))))
+     ((remove_ids3 ai a1a a2b) ()) ())
+     (fn aa =>
+       (case aa of Inl x1a => (fn () => (Inl x1a))
+         | Inr x2aa => (fn () => (Inr (SOME (a1, (x2aa, a2a)))))))
                                       else (if equal_nata a1b
          (nat_of_integer (3 : IntInf.int))
      then (fn f_ => fn () => f_ ((check_rup_proof3 ai (a1, (a1a, a2a)) a2b) ())
@@ -2109,6 +2148,1283 @@ fun verify_unsat3 x =
     end)
     x;
 
+fun backtrack3a x =
+  (fn ai => fn bi => imp_nfoldli bi (fn _ => (fn () => true)) unset_var_impl ai)
+    x;
+
+fun add_clause3a x =
+  (fn ai => fn bib => fn bia => fn (a1, a2) => fn () =>
+    let
+      val xa = array_set_dyn heap_nat zero_nat a1 bib bia ();
+      val x_b =
+        heap_WHILET
+          (fn (a1a, _) =>
+            (fn f_ => fn () => f_ ((nth heap_int ai a1a) ()) ())
+              (fn xb => (fn () => (not (equal_int xb zero_int) andalso true))))
+          (fn (a1a, a2a) =>
+            (fn f_ => fn () => f_ ((nth heap_int ai a1a) ()) ())
+              (fn x_c =>
+                (fn f_ => fn () => f_
+                  ((creg_register (equal_nat, heap_nat) x_c bib a2a) ()) ())
+                  (fn x_g => (fn () => (plus_nat one_nat a1a, x_g)))))
+          (bia, a2) ();
+    in
+      (xa, let
+             val (_, b) = x_b;
+           in
+             b
+           end)
+    end)
+    x;
+
+fun mkp_raw_err msg i p = (msg, (i, p));
+
+fun check_conflict_clause3a x =
+  (fn ai => fn bib => fn bia => fn bi => fn () =>
+    let
+      val a =
+        heap_WHILET
+          (fn a =>
+            (case a of Inl _ => (fn () => false)
+              | Inr (a1, _) =>
+                (fn f_ => fn () => f_ ((nth heap_int ai a1) ()) ())
+                  (fn xa =>
+                    (fn () => (not (equal_int xa zero_int) andalso true)))))
+          (fn s =>
+            let
+              val (a1, _) = projr s;
+            in
+              (fn f_ => fn () => f_ ((nth heap_int ai a1) ()) ())
+                (fn x_c =>
+                  (fn f_ => fn () => f_ ((op_lit_is_false_impl x_c bia) ()) ())
+                    (fn xa =>
+                      (case (if xa then Inr ()
+                              else Inl (mkp_raw_err "Expected conflict clause"
+ NONE (SOME bib)))
+                        of Inl x1a => (fn () => (Inl x1a))
+                        | Inr x2a =>
+                          (fn () => (Inr (plus_nat one_nat a1, x2a))))))
+            end)
+          (Inr (bi, ())) ();
+    in
+      (case a of Inl x1a => (fn () => (Inl x1a))
+        | Inr x2a => (fn () => (Inr let
+                                      val (_, b) = x2a;
+                                    in
+                                      b
+                                    end)))
+        ()
+    end)
+    x;
+
+fun parse_check_blocked3a x =
+  (fn ai => fn bia => fn bi => fn () =>
+    let
+      val xa = len heap_int ai ();
+    in
+      (if not (equal_nata bi xa)
+        then (fn f_ => fn () => f_
+               ((heap_WHILET
+                  (fn a =>
+                    (case a of Inl _ => (fn () => false)
+                      | Inr (a1, _) =>
+                        (fn f_ => fn () => f_ ((nth heap_int ai a1) ()) ())
+                          (fn xb =>
+                            (fn () =>
+                              (not (equal_int xb zero_int) andalso true)))))
+                  (fn s =>
+                    let
+                      val (a1, a2) = projr s;
+                    in
+                      (fn f_ => fn () => f_ ((nth heap_int ai a1) ()) ())
+                        (fn x_d =>
+                          (fn f_ => fn () => f_
+                            (let
+                               val (a1a, a2a) = a2;
+                             in
+                               (fn f_ => fn () => f_
+                                 ((op_lit_is_true_impl x_d a1a) ()) ())
+                                 (fn xb =>
+                                   (if not xb
+                                     then (fn f_ => fn () => f_
+    ((op_lit_is_false_impl x_d a1a) ()) ())
+    (fn xc =>
+      (fn f_ => fn () => f_
+        ((if xc then (fn () => (a1a, a2a))
+           else (fn f_ => fn () => f_ ((assign_lit_impl a1a (uminus_int x_d))
+                  ()) ())
+                  (fn x_j => (fn () => (x_j, (nat o abs_int) x_d :: a2a))))
+        ()) ())
+        (fn x_i => (fn () => (Inr x_i))))
+                                     else (fn () =>
+    (Inl (mkp_raw_err "Blocked lemma clause" NONE NONE)))))
+                             end
+                            ()) ())
+                            (fn a =>
+                              (case a of Inl x1a => (fn () => (Inl x1a))
+                                | Inr x2a =>
+                                  let
+                                    val x_g = plus_nat one_nat a1;
+                                  in
+                                    (fn f_ => fn () => f_ ((len heap_int ai) ())
+                                      ())
+                                      (fn xb =>
+(fn () =>
+  (if not (equal_nata x_g xb) then Inr (x_g, x2a)
+    else Inl (mkp_raw_err "Parsed beyond end" NONE NONE))))
+                                  end)))
+                    end)
+                  (Inr (bi, (bia, []))))
+               ()) ())
+               (fn a =>
+                 (case a of Inl x1a => (fn () => (Inl x1a))
+                   | Inr x2a =>
+                     (fn () =>
+                       let
+                         val ((a1a, a2a), a2) =
+                           let
+                             val (a1, a2) = let
+      val (a1, aa) = x2a;
+    in
+      (plus_nat one_nat a1, aa)
+    end;
+                           in
+                             (a2, a1)
+                           end;
+                       in
+                         Inr (bi, ((a1a, a2a), a2))
+                       end)))
+        else (fn () => (Inl (mkp_raw_err "Parsed beyond end" NONE NONE))))
+        ()
+    end)
+    x;
+
+fun check_unit_clause3a x =
+  (fn ai => fn bia => fn bi => fn () =>
+    let
+      val a =
+        heap_WHILET
+          (fn a =>
+            (case a of Inl _ => (fn () => false)
+              | Inr (a1, _) =>
+                (fn f_ => fn () => f_ ((nth heap_int ai a1) ()) ())
+                  (fn xa =>
+                    (fn () => (not (equal_int xa zero_int) andalso true)))))
+          (fn s =>
+            let
+              val (a1, a2) = projr s;
+            in
+              (fn f_ => fn () => f_ ((nth heap_int ai a1) ()) ())
+                (fn x_c =>
+                  (fn f_ => fn () => f_ ((op_lit_is_true_impl x_c bia) ()) ())
+                    (fn xa =>
+                      (if not xa
+                        then (fn f_ => fn () => f_
+                               ((op_lit_is_false_impl x_c bia) ()) ())
+                               (fn xb =>
+                                 (case (if xb then Inr a2
+ else (if equal_int zero_int a2 orelse equal_int a2 x_c then Inr x_c
+        else Inl (mkp_raw_err "2-undec in clause assumed to be unit" NONE
+                   NONE)))
+                                   of Inl x1a => (fn () => (Inl x1a))
+                                   | Inr x2a =>
+                                     (fn () =>
+                                       (Inr (plus_nat one_nat a1, x2a)))))
+                        else (fn () =>
+                               (Inl (mkp_raw_err
+                                      "True literal in clause assumed to be unit"
+                                      NONE NONE))))))
+            end)
+          (Inr (bi, zero_int)) ();
+    in
+      (case a of Inl x1a => (fn () => (Inl x1a))
+        | Inr x2a =>
+          let
+            val x_a = let
+                        val (_, b) = x2a;
+                      in
+                        b
+                      end;
+          in
+            (fn () =>
+              (if not (equal_int zero_int x_a) then Inr x_a
+                else Inl (mkp_raw_err "Conflict in clause assumed to be unit"
+                           NONE NONE)))
+          end)
+        ()
+    end)
+    x;
+
+fun parse_prf_impl prfn =
+  (fn (fuel, prf) =>
+    (if less_nat zero_nat fuel
+      then let
+             val (x, prfa) = prfn prf;
+           in
+             (fn () => (Inr (x, (minus_nat fuel one_nat, prfa))))
+           end
+      else (fn () =>
+             (Inl (mkp_raw_err "Out of fuel" NONE (SOME (fuel, prf)))))));
+
+fun resolve_id3a x =
+  (fn ai => fn bi =>
+    let
+      val (a1, _) = ai;
+    in
+      (fn () =>
+        let
+          val xa = array_get_dyn heap_nat zero_nat a1 bi ();
+        in
+          (if equal_nata zero_nat xa
+            then Inl (mkp_raw_err "Invalid clause id" (SOME (int_of_nat bi))
+                       NONE)
+            else Inr xa)
+        end)
+    end)
+    x;
+
+fun apply_units3_bta x =
+  (fn ai => fn bid => fn bic => fn bib => fn bia => fn bi => fn () =>
+    let
+      val a = parse_prf_impl bid bi ();
+    in
+      (case a of Inl x1a => (fn () => (Inl x1a))
+        | Inr x2a =>
+          (case let
+                  val (a1, a2) = x2a;
+                in
+                  (if less_eq_int zero_int a1 then Inr (nat a1, a2)
+                    else Inl (mkp_raw_err "Invalid idZ" (SOME a1) (SOME a2)))
+                end
+            of Inl x1a => (fn () => (Inl x1a))
+            | Inr (a1, a2) =>
+              (fn f_ => fn () => f_
+                ((heap_WHILET
+                   (fn aa =>
+                     (case aa of Inl _ => (fn () => false)
+                       | Inr (a1a, a2a) =>
+                         (fn () => let
+                                     val (_, _) = a1a;
+                                     val (a1c, _) = a2a;
+                                   in
+                                     not (equal_nata a1c zero_nat)
+                                   end)))
+                   (fn s =>
+                     let
+                       val ((a1b, a2b), (a1c, a2c)) = projr s;
+                     in
+                       (fn f_ => fn () => f_ ((resolve_id3a bic a1c) ()) ())
+                         (fn xa =>
+                           (fn f_ => fn () => f_
+                             ((case xa of Inl x1a => (fn () => (Inl x1a))
+                                | Inr x2ab =>
+                                  (fn f_ => fn () => f_
+                                    ((check_unit_clause3a ai a1b x2ab) ()) ())
+                                    (fn aa =>
+                                      (case aa
+of Inl x1a => (fn () => (Inl x1a))
+| Inr x2ac =>
+  (fn f_ => fn () => f_ ((assign_lit_impl a1b x2ac) ()) ())
+    (fn xb => (fn () => (Inr (xb, (nat o abs_int) x2ac :: a2b)))))))
+                             ()) ())
+                             (fn aa =>
+                               (case aa of Inl x1a => (fn () => (Inl x1a))
+                                 | Inr (a1d, a2d) =>
+                                   (fn f_ => fn () => f_
+                                     ((parse_prf_impl bid a2c) ()) ())
+                                     (fn ab =>
+                                       (case ab
+ of Inl x1a => (fn () => (Inl x1a))
+ | Inr x2ac =>
+   (case let
+           val (a1e, a2e) = x2ac;
+         in
+           (if less_eq_int zero_int a1e then Inr (nat a1e, a2e)
+             else Inl (mkp_raw_err "Invalid idZ" (SOME a1e) (SOME a2e)))
+         end
+     of Inl x1a => (fn () => (Inl x1a))
+     | Inr x2ad => (fn () => (Inr let
+                                    val (a1e, a2e) = x2ad;
+                                  in
+                                    ((a1d, a2d), (a1e, a2e))
+                                  end))))))))
+                     end)
+                   (Inr ((bib, bia), (a1, a2))))
+                ()) ())
+                (fn aa =>
+                  (case aa of Inl x1a => (fn () => (Inl x1a))
+                    | Inr (a1a, a2a) =>
+                      (fn () => let
+                                  val (a1b, a2b) = a1a;
+                                in
+                                  Inr let
+val (_, ab) = a2a;
+                                      in
+((a1b, a2b), ab)
+                                      end
+                                end)))))
+        ()
+    end)
+    x;
+
+fun check_rup_proof3a x =
+  (fn ai => fn bic => fn bib => fn bia => fn bi =>
+    let
+      val (a1, (a1a, a2a)) = bib;
+    in
+      (fn () =>
+        let
+          val a = parse_prf_impl bic bi ();
+        in
+          (case a of Inl x1a => (fn () => (Inl x1a))
+            | Inr x2a =>
+              (case let
+                      val (a1b, a2b) = x2a;
+                    in
+                      (if less_int zero_int a1b then Inr (nat a1b, a2b)
+                        else Inl (mkp_raw_err "Invalid id" (SOME a1b)
+                                   (SOME a2b)))
+                    end
+                of Inl x1a => (fn () => (Inl x1a))
+                | Inr (a1b, a2b) =>
+                  (if less_nat a1 a1b
+                    then (fn f_ => fn () => f_
+                           ((parse_check_blocked3a ai a2a bia) ()) ())
+                           (fn aa =>
+                             (case aa of Inl x1a => (fn () => (Inl x1a))
+                               | Inr (a1c, ((a1e, a2e), a2d)) =>
+                                 (fn f_ => fn () => f_
+                                   ((apply_units3_bta ai bic a1a a1e a2e a2b)
+                                   ()) ())
+                                   (fn ab =>
+                                     (case ab of Inl x1a => (fn () => (Inl x1a))
+                                       | Inr ((a1g, a2g), a2f) =>
+ (fn f_ => fn () => f_ ((parse_prf_impl bic a2f) ()) ())
+   (fn ac =>
+     (case ac of Inl x1a => (fn () => (Inl x1a))
+       | Inr x2ad =>
+         (case let
+                 val (a1h, a2h) = x2ad;
+               in
+                 (if less_int zero_int a1h then Inr (nat a1h, a2h)
+                   else Inl (mkp_raw_err "Invalid id" (SOME a1h) (SOME a2h)))
+               end
+           of Inl x1a => (fn () => (Inl x1a))
+           | Inr (a1h, a2h) =>
+             (fn f_ => fn () => f_ ((resolve_id3a a1a a1h) ()) ())
+               (fn ad =>
+                 (case ad of Inl x1a => (fn () => (Inl x1a))
+                   | Inr x2af =>
+                     (fn f_ => fn () => f_
+                       ((check_conflict_clause3a ai a2h a1g x2af) ()) ())
+                       (fn ae =>
+                         (case ae of Inl x1a => (fn () => (Inl x1a))
+                           | Inr _ =>
+                             (fn f_ => fn () => f_
+                               ((add_clause3a ai a1b a1c a1a) ()) ())
+                               (fn x_i =>
+                                 (fn f_ => fn () => f_ ((backtrack3a a1g a2g)
+                                   ()) ())
+                                   (fn x_j =>
+                                     (fn () =>
+                                       (Inr
+ ((a1b, (x_i, x_j)), (a2d, a2h)))))))))))))))))
+                    else (fn () =>
+                           (Inl (mkp_raw_err "Ids must be strictly increasing"
+                                  (SOME (int_of_nat a1b)) (SOME a2b)))))))
+            ()
+        end)
+    end)
+    x;
+
+fun and_not_C_excl3a x =
+  (fn ai => fn bib => fn bia => fn bi => fn () =>
+    let
+      val a =
+        heap_WHILET
+          (fn (a1, _) =>
+            (fn f_ => fn () => f_ ((nth heap_int ai a1) ()) ())
+              (fn xa => (fn () => (not (equal_int xa zero_int) andalso true))))
+          (fn (a1, a2) =>
+            (fn f_ => fn () => f_ ((nth heap_int ai a1) ()) ())
+              (fn x_a =>
+                (fn f_ => fn () => f_
+                  (let
+                     val (a1a, a2a) = a2;
+                   in
+                     (if not (equal_int x_a bi)
+                       then (fn f_ => fn () => f_
+                              ((op_lit_is_false_impl x_a a1a) ()) ())
+                              (fn xa =>
+                                (if not xa
+                                  then (fn f_ => fn () => f_
+ ((assign_lit_impl a1a (uminus_int x_a)) ()) ())
+ (fn x_e => (fn () => (x_e, (nat o abs_int) x_a :: a2a)))
+                                  else (fn () => (a1a, a2a))))
+                       else (fn () => (a1a, a2a)))
+                   end
+                  ()) ())
+                  (fn x_c => (fn () => (plus_nat one_nat a1, x_c)))))
+          (bia, (bib, [])) ();
+    in
+      let
+        val (_, aa) = a;
+      in
+        (fn () => aa)
+      end
+        ()
+    end)
+    x;
+
+fun check_rat_candidates_part3a x =
+  (fn ai => fn bie => fn bid => fn bic => fn bib => fn bia => fn bi => fn () =>
+    let
+      val a = parse_prf_impl bie bi ();
+    in
+      (case a of Inl x1a => (fn () => (Inl x1a))
+        | Inr x2a =>
+          (case let
+                  val (a1, a2) = x2a;
+                in
+                  (if less_eq_int zero_int a1 then Inr (nat a1, a2)
+                    else Inl (mkp_raw_err "Invalid idZ" (SOME a1) (SOME a2)))
+                end
+            of Inl x1a => (fn () => (Inl x1a))
+            | Inr (a1, a2) =>
+              (fn f_ => fn () => f_
+                ((heap_WHILET
+                   (fn aa =>
+                     (case aa of Inl _ => (fn () => false)
+                       | Inr (_, (_, (a1c, _))) =>
+                         (fn () => (not (equal_nata a1c zero_nat)))))
+                   (fn s =>
+                     let
+                       val (a1a, (a1b, (a1c, a2c))) = projr s;
+                     in
+                       (if glist_member equal_nata a1c a1a
+                         then (fn f_ => fn () => f_ ((resolve_id3a bid a1c) ())
+                                ())
+                                (fn aa =>
+                                  (case aa of Inl x1a => (fn () => (Inl x1a))
+                                    | Inr x2ab =>
+                                      (fn f_ => fn () => f_
+((and_not_C_excl3a ai a1b x2ab (uminus_int bic)) ()) ())
+(fn x_i =>
+  (fn f_ => fn () => f_
+    (let
+       val (a1d, a2d) = x_i;
+     in
+       (fn f_ => fn () => f_ ((apply_units3_bta ai bie bid a1d a2d a2c) ()) ())
+         (fn ab =>
+           (case ab of Inl x1a => (fn () => (Inl x1a))
+             | Inr ((a1f, a2f), a2e) =>
+               (fn f_ => fn () => f_ ((parse_prf_impl bie a2e) ()) ())
+                 (fn ac =>
+                   (case ac of Inl x1a => (fn () => (Inl x1a))
+                     | Inr x2ad =>
+                       (case let
+                               val (a1g, a2g) = x2ad;
+                             in
+                               (if less_int zero_int a1g then Inr (nat a1g, a2g)
+                                 else Inl
+(mkp_raw_err "Invalid id" (SOME a1g) (SOME a2g)))
+                             end
+                         of Inl x1a => (fn () => (Inl x1a))
+                         | Inr (a1g, a2g) =>
+                           (fn f_ => fn () => f_ ((resolve_id3a bid a1g) ()) ())
+                             (fn ad =>
+                               (case ad of Inl x1a => (fn () => (Inl x1a))
+                                 | Inr x2af =>
+                                   (fn f_ => fn () => f_
+                                     ((check_conflict_clause3a ai a2g a1f x2af)
+                                     ()) ())
+                                     (fn ae =>
+                                       (case ae
+ of Inl x1a => (fn () => (Inl x1a))
+ | Inr _ =>
+   (fn f_ => fn () => f_ ((backtrack3a a1f a2f) ()) ())
+     (fn x_o => (fn () => (Inr (x_o, a2g)))))))))))))
+     end
+    ()) ())
+    (fn ab =>
+      (case ab of Inl x1a => (fn () => (Inl x1a))
+        | Inr (a1d, a2d) =>
+          (fn f_ => fn () => f_ ((parse_prf_impl bie a2d) ()) ())
+            (fn ac =>
+              (case ac of Inl x1a => (fn () => (Inl x1a))
+                | Inr x2ad =>
+                  (case let
+                          val (a1e, a2e) = x2ad;
+                        in
+                          (if less_eq_int zero_int a1e then Inr (nat a1e, a2e)
+                            else Inl (mkp_raw_err "Invalid idZ" (SOME a1e)
+                                       (SOME a2e)))
+                        end
+                    of Inl x1a => (fn () => (Inl x1a))
+                    | Inr x2ae =>
+                      (fn () =>
+                        (Inr let
+                               val (a1e, a2e) = x2ae;
+                             in
+                               (glist_delete equal_nata a1c a1a,
+                                 (a1d, (a1e, a2e)))
+                             end))))))))))
+                         else (fn f_ => fn () => f_ ((parse_prf_impl bie a2c)
+                                ()) ())
+                                (fn aa =>
+                                  (case aa of Inl x1a => (fn () => (Inl x1a))
+                                    | Inr x2ab =>
+                                      (fn f_ => fn () => f_
+(let
+   val (a1d, a2d) = x2ab;
+ in
+   (fn f_ => fn () => f_
+     ((heap_WHILET
+        (fn ab =>
+          (case ab of Inl _ => (fn () => false)
+            | Inr (a1e, _) => (fn () => (not (equal_int a1e zero_int)))))
+        (fn sa => let
+                    val (_, ab) = projr sa;
+                  in
+                    parse_prf_impl bie ab
+                  end)
+        (Inr (a1d, a2d)))
+     ()) ())
+     (fn ab =>
+       (case ab of Inl x1a => (fn () => (Inl x1a))
+         | Inr x2ac => (fn () => (Inr let
+val (_, b) = x2ac;
+                                      in
+b
+                                      end))))
+ end
+()) ())
+(fn ab =>
+  (case ab of Inl x1a => (fn () => (Inl x1a))
+    | Inr x2ac =>
+      (fn f_ => fn () => f_ ((parse_prf_impl bie x2ac) ()) ())
+        (fn ac =>
+          (case ac of Inl x1a => (fn () => (Inl x1a))
+            | Inr (_, a2d) =>
+              (fn f_ => fn () => f_ ((parse_prf_impl bie a2d) ()) ())
+                (fn ad =>
+                  (case ad of Inl x1a => (fn () => (Inl x1a))
+                    | Inr x2ae =>
+                      (case let
+                              val (a1e, a2e) = x2ae;
+                            in
+                              (if less_eq_int zero_int a1e
+                                then Inr (nat a1e, a2e)
+                                else Inl (mkp_raw_err "Invalid idZ" (SOME a1e)
+   (SOME a2e)))
+                            end
+                        of Inl x1a => (fn () => (Inl x1a))
+                        | Inr x2af =>
+                          (fn () => (Inr let
+   val (a1e, a2e) = x2af;
+ in
+   (a1a, (a1b, (a1e, a2e)))
+ end))))))))))))
+                     end)
+                   (Inr (bib, (bia, (a1, a2)))))
+                ()) ())
+                (fn aa =>
+                  (case aa of Inl x1a => (fn () => (Inl x1a))
+                    | Inr (a1a, (a1b, (_, a2c))) =>
+                      (fn () =>
+                        (if is_Nil a1a then Inr (a1b, a2c)
+                          else Inl (mkp_raw_err
+                                     "Too few RAT-candidates in proof" NONE
+                                     (SOME a2c))))))))
+        ()
+    end)
+    x;
+
+fun lit_in_clause_and_not_true3a x =
+  (fn ai => fn bib => fn bia => fn bi => fn () =>
+    let
+      val xa =
+        heap_WHILET
+          (fn (a1, a2) =>
+            (fn f_ => fn () => f_ ((nth heap_int ai a1) ()) ())
+              (fn xa =>
+                (fn () =>
+                  (not (equal_int xa zero_int) andalso
+                    not (equal_nata a2 (nat_of_integer (2 : IntInf.int)))))))
+          (fn (a1, a2) =>
+            (fn f_ => fn () => f_ ((nth heap_int ai a1) ()) ())
+              (fn x_a =>
+                (fn f_ => fn () => f_
+                  ((if equal_int x_a bi then (fn () => one_nat)
+                     else (fn f_ => fn () => f_ ((op_lit_is_true_impl x_a bib)
+                            ()) ())
+                            (fn x_d =>
+                              (fn () =>
+                                (if x_d then nat_of_integer (2 : IntInf.int)
+                                  else a2))))
+                  ()) ())
+                  (fn x_c => (fn () => (plus_nat one_nat a1, x_c)))))
+          (bia, zero_nat) ();
+    in
+      equal_nata let
+                   val (_, b) = xa;
+                 in
+                   b
+                 end
+        one_nat
+    end)
+    x;
+
+fun get_rat_candidates3a x =
+  (fn ai => fn bib => fn bia => fn bi =>
+    let
+      val (a1, a2) = bib;
+      val xa = uminus_int bi;
+    in
+      (fn () =>
+        let
+          val x_b = op_creg_lookup (heap_list heap_nat) xa a2 ();
+        in
+          (if not (is_None x_b)
+            then (fn f_ => fn () => f_
+                   ((imp_nfoldli (the x_b) (fn _ => (fn () => true))
+                      (fn xh => fn sigma =>
+                        (fn f_ => fn () => f_
+                          ((array_get_dyn heap_nat zero_nat a1 xh) ()) ())
+                          (fn x_i =>
+                            (if not (equal_nata zero_nat x_i)
+                              then (fn f_ => fn () => f_
+                                     ((lit_in_clause_and_not_true3a ai bia x_i
+xa)
+                                     ()) ())
+                                     (fn x_n =>
+                                       (fn () =>
+ (if x_n then xh :: sigma else sigma)))
+                              else (fn () => sigma))))
+                      [])
+                   ()) ())
+                   (fn x_e => (fn () => (Inr x_e)))
+            else (fn () =>
+                   (Inl (mkp_raw_err "Resolution literal not declared" NONE
+                          NONE))))
+            ()
+        end)
+    end)
+    x;
+
+fun lit_in_clause3a x =
+  (fn ai => fn bia => fn bi => fn () =>
+    let
+      val a =
+        heap_WHILET
+          (fn (a1, a2) =>
+            (fn f_ => fn () => f_ ((nth heap_int ai a1) ()) ())
+              (fn xa =>
+                (fn () => (not (equal_int xa zero_int) andalso not a2))))
+          (fn (a1, _) =>
+            (fn f_ => fn () => f_ ((nth heap_int ai a1) ()) ())
+              (fn x_a => (fn () => (plus_nat one_nat a1, equal_int bi x_a))))
+          (bia, false) ();
+    in
+      let
+        val (_, aa) = a;
+      in
+        (fn () => aa)
+      end
+        ()
+    end)
+    x;
+
+fun check_rat_proof3a x =
+  (fn ai => fn bic => fn bib => fn bia => fn bi =>
+    let
+      val (a1, (a1a, a2a)) = bib;
+    in
+      (fn () =>
+        let
+          val a = parse_prf_impl bic bi ();
+        in
+          (case a of Inl x1a => (fn () => (Inl x1a))
+            | Inr x2a =>
+              (case let
+                      val (a1b, a2b) = x2a;
+                    in
+                      (if not (equal_int a1b zero_int) then Inr (a1b, a2b)
+                        else Inl (mkp_raw_err "Expected literal but found 0"
+                                   NONE (SOME a2b)))
+                    end
+                of Inl x1a => (fn () => (Inl x1a))
+                | Inr (a1b, a2b) =>
+                  (fn f_ => fn () => f_ ((op_lit_is_false_impl a1b a2a) ()) ())
+                    (fn xa =>
+                      (if not xa
+                        then (fn f_ => fn () => f_ ((parse_prf_impl bic a2b) ())
+                               ())
+                               (fn aa =>
+                                 (case aa of Inl x1a => (fn () => (Inl x1a))
+                                   | Inr x2ab =>
+                                     (case let
+     val (a1c, a2c) = x2ab;
+   in
+     (if less_int zero_int a1c then Inr (nat a1c, a2c)
+       else Inl (mkp_raw_err "Invalid id" (SOME a1c) (SOME a2c)))
+   end
+                                       of Inl x1a => (fn () => (Inl x1a))
+                                       | Inr (a1c, a2c) =>
+ (if less_nat a1 a1c
+   then (fn f_ => fn () => f_ ((parse_check_blocked3a ai a2a bia) ()) ())
+          (fn ab =>
+            (case ab of Inl x1a => (fn () => (Inl x1a))
+              | Inr (a1d, ((a1f, a2f), a2e)) =>
+                (fn f_ => fn () => f_ ((lit_in_clause3a ai a1d a1b) ()) ())
+                  (fn x_g =>
+                    (case (if x_g then Inr ()
+                            else Inl (mkp_raw_err
+                                       "Resolution literal not in clause" NONE
+                                       (SOME a2c)))
+                      of Inl x1a => (fn () => (Inl x1a))
+                      | Inr _ =>
+                        (fn f_ => fn () => f_
+                          ((apply_units3_bta ai bic a1a a1f a2f a2c) ()) ())
+                          (fn ac =>
+                            (case ac of Inl x1a => (fn () => (Inl x1a))
+                              | Inr ((a1h, a2h), a2g) =>
+                                (fn f_ => fn () => f_
+                                  ((get_rat_candidates3a ai a1a a1h a1b) ()) ())
+                                  (fn ad =>
+                                    (case ad of Inl x1a => (fn () => (Inl x1a))
+                                      | Inr x2ag =>
+(fn f_ => fn () => f_ ((check_rat_candidates_part3a ai bic a1a a1b x2ag a1h a2g)
+  ()) ())
+  (fn ae =>
+    (case ae of Inl x1a => (fn () => (Inl x1a))
+      | Inr x2ah =>
+        (fn f_ => fn () => f_
+          (let
+             val (a1i, a2i) = x2ah;
+           in
+             (fn f_ => fn () => f_ ((add_clause3a ai a1c a1d a1a) ()) ())
+               (fn x_l =>
+                 (fn f_ => fn () => f_ ((backtrack3a a1i a2h) ()) ())
+                   (fn x_m => (fn () => ((a1c, (x_l, x_m)), (a2e, a2i)))))
+           end
+          ()) ())
+          (fn x_l => (fn () => (Inr x_l)))))))))))))
+   else (fn () =>
+          (Inl (mkp_raw_err "Ids must be strictly increasing"
+                 (SOME (int_of_nat a1c)) (SOME a2c))))))))
+                        else (fn () =>
+                               (Inl (mkp_raw_err "Resolution literal is false"
+                                      NONE (SOME a2b))))))))
+            ()
+        end)
+    end)
+    x;
+
+fun apply_units3a x =
+  (fn ai => fn bic => fn bib => fn bia => fn bi => fn () =>
+    let
+      val a = parse_prf_impl bic bi ();
+    in
+      (case a of Inl x1a => (fn () => (Inl x1a))
+        | Inr x2a =>
+          (case let
+                  val (a1, a2) = x2a;
+                in
+                  (if less_eq_int zero_int a1 then Inr (nat a1, a2)
+                    else Inl (mkp_raw_err "Invalid idZ" (SOME a1) (SOME a2)))
+                end
+            of Inl x1a => (fn () => (Inl x1a))
+            | Inr (a1, a2) =>
+              (fn f_ => fn () => f_
+                ((heap_WHILET
+                   (fn aa =>
+                     (case aa of Inl _ => (fn () => false)
+                       | Inr (_, (a1b, _)) =>
+                         (fn () => (not (equal_nata a1b zero_nat)))))
+                   (fn s =>
+                     let
+                       val (a1a, (a1b, a2b)) = projr s;
+                     in
+                       (fn f_ => fn () => f_ ((resolve_id3a bib a1b) ()) ())
+                         (fn xa =>
+                           (fn f_ => fn () => f_
+                             ((case xa of Inl x1a => (fn () => (Inl x1a))
+                                | Inr x2ab =>
+                                  (fn f_ => fn () => f_
+                                    ((check_unit_clause3a ai a1a x2ab) ()) ())
+                                    (fn aa =>
+                                      (case aa
+of Inl x1a => (fn () => (Inl x1a))
+| Inr x2ac =>
+  (fn f_ => fn () => f_ ((assign_lit_impl a1a x2ac) ()) ())
+    (fn x_g => (fn () => (Inr x_g))))))
+                             ()) ())
+                             (fn aa =>
+                               (case aa of Inl x1a => (fn () => (Inl x1a))
+                                 | Inr x2ab =>
+                                   (fn f_ => fn () => f_
+                                     ((parse_prf_impl bic a2b) ()) ())
+                                     (fn ab =>
+                                       (case ab
+ of Inl x1a => (fn () => (Inl x1a))
+ | Inr x2ac =>
+   (case let
+           val (a1c, a2c) = x2ac;
+         in
+           (if less_eq_int zero_int a1c then Inr (nat a1c, a2c)
+             else Inl (mkp_raw_err "Invalid idZ" (SOME a1c) (SOME a2c)))
+         end
+     of Inl x1a => (fn () => (Inl x1a))
+     | Inr x2ad => (fn () => (Inr let
+                                    val (a1c, a2c) = x2ad;
+                                  in
+                                    (x2ab, (a1c, a2c))
+                                  end))))))))
+                     end)
+                   (Inr (bia, (a1, a2))))
+                ()) ())
+                (fn aa =>
+                  (case aa of Inl x1a => (fn () => (Inl x1a))
+                    | Inr x2ab => (fn () => (Inr let
+           val (a1a, ab) = x2ab;
+           val (_, ac) = ab;
+         in
+           (a1a, ac)
+         end))))))
+        ()
+    end)
+    x;
+
+fun remove_ids3a x =
+  (fn ai => fn bia => fn bi => fn () =>
+    let
+      val a = parse_prf_impl ai bi ();
+    in
+      (case a of Inl x1a => (fn () => (Inl x1a))
+        | Inr x2a =>
+          (case let
+                  val (a1, a2) = x2a;
+                in
+                  (if less_eq_int zero_int a1 then Inr (nat a1, a2)
+                    else Inl (mkp_raw_err "Invalid idZ" (SOME a1) (SOME a2)))
+                end
+            of Inl x1a => (fn () => (Inl x1a))
+            | Inr (a1, a2) =>
+              (fn f_ => fn () => f_
+                ((heap_WHILET
+                   (fn aa =>
+                     (case aa of Inl _ => (fn () => false)
+                       | Inr (_, (a1b, _)) =>
+                         (fn () => (not (equal_nata a1b zero_nat)))))
+                   (fn s =>
+                     let
+                       val (a1a, (a1b, a2b)) = projr s;
+                     in
+                       (fn f_ => fn () => f_
+                         (let
+                            val (a1c, a2c) = a1a;
+                          in
+                            (fn f_ => fn () => f_
+                              ((array_set_dyn heap_nat zero_nat a1c a1b
+                                 zero_nat)
+                              ()) ())
+                              (fn x_e => (fn () => (x_e, a2c)))
+                          end
+                         ()) ())
+                         (fn x_e =>
+                           (fn f_ => fn () => f_ ((parse_prf_impl ai a2b) ())
+                             ())
+                             (fn aa =>
+                               (case aa of Inl x1a => (fn () => (Inl x1a))
+                                 | Inr x2ab =>
+                                   (case let
+   val (a1c, a2c) = x2ab;
+ in
+   (if less_eq_int zero_int a1c then Inr (nat a1c, a2c)
+     else Inl (mkp_raw_err "Invalid idZ" (SOME a1c) (SOME a2c)))
+ end
+                                     of Inl x1a => (fn () => (Inl x1a))
+                                     | Inr x2ac =>
+                                       (fn () =>
+ (Inr let
+        val (a1c, a2c) = x2ac;
+      in
+        (x_e, (a1c, a2c))
+      end))))))
+                     end)
+                   (Inr (bia, (a1, a2))))
+                ()) ())
+                (fn aa =>
+                  (case aa of Inl x1a => (fn () => (Inl x1a))
+                    | Inr x2ab => (fn () => (Inr let
+           val (a1a, ab) = x2ab;
+           val (_, ac) = ab;
+         in
+           (a1a, ac)
+         end))))))
+        ()
+    end)
+    x;
+
+fun check_item3a x =
+  (fn ai => fn bic => fn bib => fn bia => fn bi =>
+    let
+      val (a1, (a1a, a2a)) = bib;
+    in
+      (fn () =>
+        let
+          val a = parse_prf_impl bic bi ();
+        in
+          (case a of Inl x1a => (fn () => (Inl x1a))
+            | Inr (a1b, a2b) =>
+              (if equal_int a1b (Int_of_integer (1 : IntInf.int))
+                then (fn f_ => fn () => f_ ((apply_units3a ai bic a1a a2a a2b)
+                       ()) ())
+                       (fn aa =>
+                         (case aa of Inl x1a => (fn () => (Inl x1a))
+                           | Inr x2aa =>
+                             (fn () =>
+                               (Inr let
+                                      val (a1c, a2c) = x2aa;
+                                    in
+                                      SOME ((a1, (a1a, a1c)), (bia, a2c))
+                                    end))))
+                else (if equal_int a1b (Int_of_integer (2 : IntInf.int))
+                       then (fn f_ => fn () => f_ ((remove_ids3a bic a1a a2b)
+                              ()) ())
+                              (fn aa =>
+                                (case aa of Inl x1a => (fn () => (Inl x1a))
+                                  | Inr x2aa =>
+                                    (fn () =>
+                                      (Inr
+let
+  val (a1c, a2c) = x2aa;
+in
+  SOME ((a1, (a1c, a2a)), (bia, a2c))
+end))))
+                       else (if equal_int a1b (Int_of_integer (3 : IntInf.int))
+                              then (fn f_ => fn () => f_
+                                     ((check_rup_proof3a ai bic (a1, (a1a, a2a))
+bia a2b)
+                                     ()) ())
+                                     (fn aa =>
+                                       (case aa
+ of Inl x1a => (fn () => (Inl x1a)) | Inr x2aa => (fn () => (Inr (SOME x2aa)))))
+                              else (if equal_int a1b
+ (Int_of_integer (4 : IntInf.int))
+                                     then (fn f_ => fn () => f_
+    ((check_rat_proof3a ai bic (a1, (a1a, a2a)) bia a2b) ()) ())
+    (fn aa =>
+      (case aa of Inl x1a => (fn () => (Inl x1a))
+        | Inr x2aa => (fn () => (Inr (SOME x2aa)))))
+                                     else (if equal_int a1b
+        (Int_of_integer (5 : IntInf.int))
+    then (fn f_ => fn () => f_ ((parse_prf_impl bic a2b) ()) ())
+           (fn aa =>
+             (case aa of Inl x1a => (fn () => (Inl x1a))
+               | Inr x2aa =>
+                 (case let
+                         val (a1c, a2c) = x2aa;
+                       in
+                         (if less_int zero_int a1c then Inr (nat a1c, a2c)
+                           else Inl (mkp_raw_err "Invalid id" (SOME a1c)
+                                      (SOME a2c)))
+                       end
+                   of Inl x1a => (fn () => (Inl x1a))
+                   | Inr (a1c, a2c) =>
+                     (fn f_ => fn () => f_ ((resolve_id3a a1a a1c) ()) ())
+                       (fn ab =>
+                         (case ab of Inl x1a => (fn () => (Inl x1a))
+                           | Inr x2ac =>
+                             (fn f_ => fn () => f_
+                               ((check_conflict_clause3a ai a2c a2a x2ac) ())
+                               ())
+                               (fn ac =>
+                                 (case ac of Inl x1a => (fn () => (Inl x1a))
+                                   | Inr _ => (fn () => (Inr NONE)))))))))
+    else (fn () =>
+           (if equal_int a1b (Int_of_integer (6 : IntInf.int))
+             then Inl (mkp_raw_err
+                        "Not expecting rat-counts in the middle of proof" NONE
+                        (SOME a2b))
+             else Inl (mkp_raw_err "Invalid item type" (SOME a1b)
+                        (SOME a2b))))))))))
+            ()
+        end)
+    end)
+    x;
+
+fun read_clause_check_taut3a x =
+  (fn ai => fn bib => fn bia => fn bi =>
+    (if not (equal_nata bia bib)
+      then (fn () =>
+             let
+               val a =
+                 heap_WHILET
+                   (fn a =>
+                     (case a of Inl _ => (fn () => false)
+                       | Inr (a1, _) =>
+                         (fn f_ => fn () => f_ ((nth heap_int ai a1) ()) ())
+                           (fn xa =>
+                             (fn () =>
+                               (not (equal_int xa zero_int) andalso true)))))
+                   (fn s =>
+                     let
+                       val (a1, a2) = projr s;
+                     in
+                       (fn f_ => fn () => f_ ((nth heap_int ai a1) ()) ())
+                         (fn x_d =>
+                           (fn f_ => fn () => f_
+                             (let
+                                val (a1a, a2a) = a2;
+                              in
+                                (fn f_ => fn () => f_
+                                  ((op_lit_is_false_impl x_d a2a) ()) ())
+                                  (fn x_h =>
+                                    (if x_h then (fn () => (true, a2a))
+                                      else (fn f_ => fn () => f_
+     ((assign_lit_impl a2a x_d) ()) ())
+     (fn x_i => (fn () => (a1a, x_i)))))
+                              end
+                             ()) ())
+                             (fn x_f =>
+                               let
+                                 val x_g = plus_nat one_nat a1;
+                               in
+                                 (fn () =>
+                                   (if not (equal_nata x_g bib)
+                                     then Inr (x_g, x_f)
+                                     else Inl
+    (mkp_raw_err "Parsed beyond end" NONE NONE)))
+                               end))
+                     end)
+                   (Inr (bia, (false, bi))) ();
+             in
+               (case a of Inl x1a => (fn () => (Inl x1a))
+                 | Inr x2a =>
+                   (fn f_ => fn () => f_
+                     (let
+                        val (a1, (a1a, a2a)) = let
+         val (a1, aa) = x2a;
+       in
+         (plus_nat one_nat a1, aa)
+       end;
+                      in
+                        (fn f_ => fn () => f_
+                          ((heap_WHILET
+                             (fn (a1b, _) =>
+                               (fn f_ => fn () => f_ ((nth heap_int ai a1b) ())
+                                 ())
+                                 (fn xa =>
+                                   (fn () =>
+                                     (not (equal_int xa zero_int) andalso
+                                       true))))
+                             (fn (a1b, a2b) =>
+                               (fn f_ => fn () => f_ ((nth heap_int ai a1b) ())
+                                 ())
+                                 (fn x_d =>
+                                   (fn f_ => fn () => f_
+                                     ((unset_var_impl ((nat o abs_int) x_d) a2b)
+                                     ()) ())
+                                     (fn x_f =>
+                                       (fn () => (plus_nat one_nat a1b, x_f)))))
+                             (bia, a2a))
+                          ()) ())
+                          (fn x_c =>
+                            (fn () => (a1, (a1a, let
+           val (_, b) = x_c;
+         in
+           b
+         end))))
+                      end
+                     ()) ())
+                     (fn x_c => (fn () => (Inr x_c))))
+                 ()
+             end)
+      else (fn () => (Inl (mkp_raw_err "Parsed beyond end" NONE NONE)))))
+    x;
+
+fun read_cnf_new3a x =
+  (fn ai => fn bib => fn bia => fn bi => fn () =>
+    let
+      val xa = assignment_empty_impl ();
+      val a =
+        heap_WHILET
+          (fn a =>
+            (case a of Inl _ => (fn () => false)
+              | Inr (a1, _) => (fn () => (not (equal_nata a1 bib)))))
+          (fn s =>
+            let
+              val (a1, (a1a, (a1b, a2b))) = projr s;
+            in
+              (fn f_ => fn () => f_ ((read_clause_check_taut3a ai bib a1 a2b)
+                ()) ())
+                (fn a =>
+                  (case a of Inl x1a => (fn () => (Inl x1a))
+                    | Inr x2a =>
+                      (fn f_ => fn () => f_
+                        ((case x2a
+                           of (a1c, (true, a2d)) =>
+                             (fn () =>
+                               (a1c, (a1a, (plus_nat a1b one_nat, a2d))))
+                           | (a1c, (false, a2d)) =>
+                             (fn f_ => fn () => f_ ((add_clause3a ai a1b a1 a1a)
+                               ()) ())
+                               (fn x_e =>
+                                 (fn () =>
+                                   (a1c, (x_e, (plus_nat a1b one_nat, a2d))))))
+                        ()) ())
+                        (fn x_d => (fn () => (Inr x_d)))))
+            end)
+          (Inr (bia, (bi, (one_nat, xa)))) ();
+    in
+      (case a of Inl x1a => (fn () => (Inl x1a))
+        | Inr x2a =>
+          (fn () => (Inr let
+                           val (a1, (a1a, _)) = let
+          val (_, b) = x2a;
+        in
+          b
+        end;
+                         in
+                           (a1, minus_nat a1a one_nat)
+                         end)))
+        ()
+    end)
+    x;
+
+fun init_rat_counts3a x =
+  (fn ai => fn bi => fn () =>
+    let
+      val a = parse_prf_impl ai bi ();
+    in
+      (case a of Inl x1a => (fn () => (Inl x1a))
+        | Inr (a1, a2) =>
+          (if equal_int a1 (Int_of_integer (1 : IntInf.int)) orelse
+                (equal_int a1 (Int_of_integer (2 : IntInf.int)) orelse
+                  (equal_int a1 (Int_of_integer (3 : IntInf.int)) orelse
+                    (equal_int a1 (Int_of_integer (4 : IntInf.int)) orelse
+                      (equal_int a1 (Int_of_integer (5 : IntInf.int)) orelse
+                        equal_int a1 (Int_of_integer (6 : IntInf.int))))))
+            then (if equal_int a1 (Int_of_integer (6 : IntInf.int))
+                   then (fn f_ => fn () => f_ ((parse_prf_impl ai a2) ()) ())
+                          (fn aa =>
+                            (case aa of Inl x1a => (fn () => (Inl x1a))
+                              | Inr x2aa =>
+                                let
+                                  val (a1a, a2a) =
+                                    let
+                                      val (a1a, a2a) = x2aa;
+                                    in
+                                      (if equal_int a1a zero_int
+then (zero_int, a2a) else (a1a, a2a))
+                                    end;
+                                in
+                                  (fn f_ => fn () => f_
+                                    ((new heap_nat
+                                       (nat_of_integer (16 : IntInf.int))
+                                       zero_nat)
+                                    ()) ())
+                                    (fn xa =>
+                                      (fn f_ => fn () => f_ (creg_empty ()) ())
+(fn xaa =>
+  (fn f_ => fn () => f_
+    ((heap_WHILET
+       (fn ab =>
+         (case ab of Inl _ => (fn () => false)
+           | Inr (_, (a1c, _)) => (fn () => (not (equal_int zero_int a1c)))))
+       (fn s =>
+         let
+           val (a1b, (a1c, a2c)) = projr s;
+         in
+           (fn f_ => fn () => f_ ((parse_prf_impl ai a2c) ()) ())
+             (fn ab =>
+               (case ab of Inl x1a => (fn () => (Inl x1a))
+                 | Inr (_, a2d) =>
+                   (fn f_ => fn () => f_
+                     (let
+                        val (a1e, a2e) = a1b;
+                      in
+                        (fn f_ => fn () => f_
+                          ((creg_initialize (uminus_int a1c) a2e) ()) ())
+                          (fn x_m => (fn () => (a1e, x_m)))
+                      end
+                     ()) ())
+                     (fn x_m =>
+                       (fn f_ => fn () => f_ ((parse_prf_impl ai a2d) ()) ())
+                         (fn ac =>
+                           (case ac of Inl x1a => (fn () => (Inl x1a))
+                             | Inr x2ac =>
+                               (fn () =>
+                                 (Inr let
+val (a1e, a2e) =
+  let
+    val (a1e, a2e) = x2ac;
+  in
+    (if equal_int a1e zero_int then (zero_int, a2e) else (a1e, a2e))
+  end;
+                                      in
+(x_m, (a1e, a2e))
+                                      end)))))))
+         end)
+       (Inr ((xa, xaa), (a1a, a2a))))
+    ()) ())
+    (fn ab =>
+      (case ab of Inl x1a => (fn () => (Inl x1a))
+        | Inr x2ab => (fn () => (Inr let
+                                       val (a1b, ac) = x2ab;
+                                       val (_, ad) = ac;
+                                     in
+                                       (a1b, ad)
+                                     end))))))
+                                end))
+                   else (fn () =>
+                          (Inl (mkp_raw_err "Expected RAT counts item" NONE
+                                 (SOME a2)))))
+            else (fn () =>
+                   (Inl (mkp_raw_err "Invalid item type" (SOME a1)
+                          (SOME a2))))))
+        ()
+    end)
+    x;
+
+fun verify_unsat3a x =
+  (fn ai => fn bid => fn bic => fn bib => fn bia => fn bi => fn () =>
+    let
+      val xa = assignment_empty_impl ();
+      val a = init_rat_counts3a bid bi ();
+    in
+      (case a of Inl x1a => (fn () => (Inl x1a))
+        | Inr (a1, a2) =>
+          (fn f_ => fn () => f_ ((read_cnf_new3a ai bib bic a1) ()) ())
+            (fn aa =>
+              (case aa of Inl x1a => (fn () => (Inl x1a))
+                | Inr (a1a, a2a) =>
+                  (fn f_ => fn () => f_
+                    ((heap_WHILET
+                       (fn ab =>
+                         (case ab of Inl _ => (fn () => false)
+                           | Inr x2ab => (fn () => (not (is_None x2ab)))))
+                       (fn s => let
+                                  val (a1b, ab) = the (projr s);
+                                  val (ac, b) = ab;
+                                in
+                                  check_item3a ai bid a1b ac b
+                                end)
+                       (Inr (SOME ((a2a, (a1a, xa)), (bia, a2)))))
+                    ()) ())
+                    (fn ab =>
+                      (case ab of Inl x1a => (fn () => (Inl x1a))
+                        | Inr x2ab =>
+                          (fn () =>
+                            (if is_None x2ab then Inr ()
+                              else Inl (mkp_raw_err
+ "Proof did not contain conflict declaration" NONE NONE))))))))
+        ()
+    end)
+    x;
+
 fun verify_sat_impl_wrapper dBi f_end =
   (fn () =>
     let
@@ -2129,6 +3445,19 @@ fun verify_unsat_impl_wrapper dBi f_end it =
             (less_eq_nat f_end lenDBi andalso
               (less_nat zero_nat it andalso less_eq_nat it lenDBi))
         then verify_unsat3 dBi f_end one_nat f_end it
+        else (fn () => (Inl ("Invalid arguments", (NONE, NONE)))))
+        ()
+    end);
+
+fun verify_unsat_split_impl_wrapper dBi prf_next f_end it prf =
+  (fn () =>
+    let
+      val lenDBi = len heap_int dBi ();
+    in
+      (if less_nat zero_nat f_end andalso
+            (less_eq_nat f_end lenDBi andalso
+              (less_nat zero_nat it andalso less_eq_nat it lenDBi))
+        then verify_unsat3a dBi prf_next one_nat f_end it prf
         else (fn () => (Inl ("Invalid arguments", (NONE, NONE)))))
         ()
     end);
