GRAT/gratgen/doc/html/search/all_b.js
@@ -1,6 +1,7 @@
 var searchData=
 [
   ['main',['main',['../gratgen_8cpp.html#a3c04138a5bfe5d72780bb7e82a18e627',1,'gratgen.cpp']]],
-  ['mark_5fclause',['mark_clause',['../classSynch__Data.html#a023af3c79d4618efec7271b01b36ff9f',1,'Synch_Data::mark_clause()'],['../classVerifier.html#ac0d4d56e1dce70d5aa88e9d8783fc252',1,'Verifier::mark_clause()']]],
+  ['mark_5fclause',['mark_clause',['../classVerifier.html#ac0d4d56e1dce70d5aa88e9d8783fc252',1,'Verifier']]],
+  ['mark_5fclause_5fsingle_5fthreaded',['mark_clause_single_threaded',['../classSynch__Data.html#a95c51ad5378eb87cbcb5e1e2497ddf48',1,'Synch_Data']]],
   ['mark_5fvar',['mark_var',['../classVerifier.html#a38eb63fca984901cf62592f201c90f80',1,'Verifier']]]
 ];
