GRAT/ToolPaper/massage_snippets.sed
@@ -1,0 +1,3 @@
+# TODO: Can be done at isabelle level, look at LaTeXSugar for example!
+s/([^a-zA-Z{])(spec|case|while|selectp|return|do|let)([^a-zA-Z}])/\1\\isainnerkeyword{\2}\3/g;
+s/\{\\isasymexists\}\\isactrlsub A/{\\isasymexistsA}/g;
