GRAT/evaluation/integrate.gawk
@@ -1,0 +1,21 @@
+#!/usr/bin/gawk -f
+
+BEGIN {
+  count=0
+  last=0
+}
+
+{
+  this=$1
+  
+  if (this>last && last!=0) {
+    print count "\t " last 
+  }
+
+  last=this
+  count++
+}
+
+END {
+  print count "\t " last 
+}
